src/Rupicola/Lib/Core.v
@@ -1085,12 +1085,14 @@ Module word.
     End MinMax.
 
     Ltac compile_binop_zzw_bitwise lemma :=
-      intros; cbn;
-      apply word.unsigned_inj;
-      rewrite lemma, !word.unsigned_of_Z;
-      bitblast.Z.bitblast;
-      rewrite !word.testbit_wrap;
-      bitblast.Z.bitblast_core.
+      intros; cbn; apply word.unsigned_inj;
+      rewrite lemma, !word.unsigned_of_Z by lia;
+      unfold word.wrap; rewrite <- ?Z.land_ones by eauto using word.width_nonneg;
+      bitblast.Z.bitblast.
+
+    Lemma morph_not x :
+      word.of_Z (Z.lnot x) = word.not (word.of_Z x) :> word.
+    Proof. compile_binop_zzw_bitwise word.unsigned_not. Qed.
 
     Lemma morph_and x y:
       word.of_Z (Z.land x y) = word.and (word.of_Z x) (word.of_Z y) :> word.
@@ -1103,6 +1105,14 @@ Module word.
     Lemma morph_xor x y:
       word.of_Z (Z.lxor x y) = word.xor (word.of_Z x) (word.of_Z y) :> word.
     Proof. compile_binop_zzw_bitwise word.unsigned_xor_nowrap. Qed.
+
+    Lemma morph_shiftl z n:
+      0 <= n < width ->
+      word.of_Z (Z.shiftl z n) = word.slu (word := word) (word.of_Z z) (word.of_Z n).
+    Proof.
+      compile_binop_zzw_bitwise word.unsigned_slu_shamtZ.
+      rewrite ?Z.testbit_neg_r by assumption; reflexivity.
+    Qed.
 
     Lemma Z_land_wrap_l z1 z2:
       0 <= z2 < 2 ^ width ->
@@ -1122,6 +1132,48 @@ Module word.
     Proof.
       intros; rewrite Z.land_comm at 1;
         rewrite Z_land_wrap_l by lia; apply Z.land_comm.
+    Qed.
+
+    Lemma of_Z_land_ones z :
+      word.of_Z (Z.land z (Z.ones width)) = word.of_Z (word := word) z.
+    Proof.
+      rewrite Z.land_ones by apply word.width_nonneg.
+      apply word.unsigned_inj; rewrite !word.unsigned_of_Z; unfold word.wrap.
+      Z.push_pull_mod; reflexivity.
+    Qed.
+
+    Lemma Z_land_ones_word_add (a b: word) :
+      Z.land (word.unsigned a + word.unsigned b) (Z.ones width) =
+        word.unsigned (word.add a b).
+    Proof. rewrite Z.land_ones, word.unsigned_add; reflexivity || apply word.width_nonneg. Qed.
+
+    Lemma Z_land_ones_rotate (a: word) b (Hrange: 0 < b < width) :
+      Z.land (Z.shiftl (word.unsigned a) b + Z.shiftr (word.unsigned a) (width - b)) (Z.ones width) =
+        word.unsigned (word.add (word.slu a (word.of_Z b)) (word.sru a (word.sub (word.of_Z width) (word.of_Z b)))).
+    Proof.
+      rewrite Z.land_ones, word.unsigned_add by lia.
+      rewrite word.unsigned_slu, word.unsigned_sru, !word.unsigned_of_Z_nowrap.
+      unfold word.wrap; Z.push_pull_mod.
+      rewrite word.unsigned_sub, !word.unsigned_of_Z, !wrap_small.
+      reflexivity.
+      all: pose proof Zpow_facts.Zpower2_lt_lin width word.width_nonneg.
+      all: rewrite ?word.unsigned_sub, ?word.unsigned_of_Z_nowrap, ?wrap_small; lia.
+    Qed.
+
+    Lemma of_Z_land_ones_rotate a b (Ha: 0 <= a < 2 ^ width) (Hb: 0 < b < width) :
+      word.of_Z (Z.land (Z.shiftl a b + Z.shiftr a (width - b)) (Z.ones width)) =
+        word.add (word := word)
+                 (word.slu (word.of_Z a) (word.of_Z b))
+                 (word.sru (word.of_Z a) (word.sub (word.of_Z width) (word.of_Z b))).
+    Proof.
+      apply word.unsigned_inj.
+      rewrite word.unsigned_add, word.unsigned_slu, word.unsigned_sru_nowrap;
+        rewrite ?word.unsigned_sub, ?word.unsigned_of_Z_nowrap.
+      all: rewrite ?(wrap_small b), ?(wrap_small (width - b)).
+      unfold word.wrap; rewrite Z.land_ones by apply word.width_nonneg;
+        Z.push_pull_mod; reflexivity.
+      all: pose proof Zpow_facts.Zpower2_lt_lin width word.width_nonneg; try lia.
+      rewrite Z.land_ones by lia; apply Z.mod_pos_bound; lia.
     Qed.
   End __.
 End word.
@@ -1331,6 +1383,340 @@ Section Scalar.
   Qed.
 End Scalar.
 
+Section Byte.
+  Lemma testbit_byte_unsigned_ge b n:
+    8 <= n ->
+    Z.testbit (byte.unsigned b) n = false.
+  Proof.
+    intros;
+      erewrite prove_Zeq_bitwise.testbit_above;
+      eauto using byte.unsigned_range;
+      lia.
+  Qed.
+
+  (* FIXME this doesn't do anything *)
+  Hint Rewrite testbit_byte_unsigned_ge using solve [auto with zarith] : z_bitwise_with_hyps.
+
+  (* FIXME isn't this defined somewhere already? *)
+  Definition byte_land (b1 b2: byte) :=
+    byte.of_Z (Z.land (byte.unsigned b1) (byte.unsigned b2)).
+
+  Lemma byte_unsigned_land (b1 b2: byte) :
+    byte.unsigned (byte_land b1 b2) =
+      Z.land (byte.unsigned b1) (byte.unsigned b2).
+  Proof.
+    unfold byte_land; rewrite byte.unsigned_of_Z.
+    unfold byte.wrap; rewrite <- Z.land_ones.
+    bitblast.Z.bitblast.
+    rewrite testbit_byte_unsigned_ge.
+    all: lia.
+  Qed.
+
+  Lemma byte_xor_comm b1 b2:
+    byte.xor b1 b2 = byte.xor b2 b1.
+  Proof. unfold byte.xor; rewrite Z.lxor_comm; reflexivity. Qed.
+End Byte.
+
+Ltac div_up_t :=
+  cbv [Nat.div_up]; zify;
+  rewrite ?Zdiv.div_Zdiv, ?mod_Zmod in * by Lia.lia;
+  Z.div_mod_to_equations;
+  nia.
+
+Section DivUp.
+  Lemma div_up_eqn a b:
+    Nat.div_up a b =
+    (a / b + if a mod b =? 0 then 0 else 1)%nat.
+  Proof.
+    destruct (Nat.eq_dec b 0); [ subst; reflexivity | ].
+    destruct (Nat.eqb_spec (a mod b) 0); div_up_t.
+  Qed.
+
+  Lemma div_up_add_mod a b n:
+    (a mod n = 0)%nat ->
+    Nat.div_up (a + b) n =
+    (Nat.div_up a n + Nat.div_up b n)%nat.
+  Proof.
+    intros; destruct (Nat.eq_dec n 0); subst; [ reflexivity | ].
+    rewrite !div_up_eqn.
+    rewrite <- Nat.add_mod_idemp_l by assumption.
+    replace (a mod n)%nat; cbn [Nat.add Nat.eqb].
+    rewrite (Nat.div_mod a n) by assumption.
+    replace (a mod n)%nat; cbn [Nat.add Nat.eqb].
+    rewrite !Nat.add_0_r, !(Nat.mul_comm n (a/n)).
+    rewrite !Nat.div_add_l, !Nat.div_mul by assumption.
+    lia.
+  Qed.
+
+  Lemma div_up_exact a b:
+    (b <> 0)%nat ->
+    (a mod b = 0)%nat <->
+    (a = b * (Nat.div_up a b))%nat.
+  Proof.
+    intros.
+    rewrite div_up_eqn.
+    split; intros Heq.
+    - rewrite Heq; cbn; rewrite Nat.mul_add_distr_l, Nat.mul_0_r, Nat.add_0_r.
+      apply Nat.div_exact; assumption.
+    - replace a; rewrite Nat.mul_comm; apply Nat.mod_mul; assumption.
+  Qed.
+
+  Lemma div_up_exact_mod a b:
+    (b <> 0)%nat ->
+    (a mod b = 0)%nat ->
+    ((Nat.div_up a b) * b = a)%nat.
+  Proof. intros * H0 Hmod; eapply div_up_exact in Hmod; lia. Qed.
+End DivUp.
+
+Section Chunks.
+  Lemma Forall_chunk'_length_mod {A} (l: list A) n:
+    forall acc, (length acc < n)%nat ->
+           ((length l + length acc) mod n = length l mod n)%nat ->
+           Forall (fun c => length c = n \/ length c = length l mod n)%nat
+                  (chunk' n l acc).
+  Proof.
+    set (length l) as ll at 2 3; clearbody ll.
+    induction l; simpl; intros.
+    - destruct acc; eauto; [].
+      apply Forall_cons; eauto.
+      right. rewrite <- (Nat.mod_small _ n); assumption.
+    - destruct (_ <? _)%nat eqn:Hlt.
+      + rewrite Nat.ltb_lt in Hlt.
+        eapply IHl; try lia; [].
+        rewrite app_length; cbn [List.length].
+        replace (ll mod n)%nat; f_equal; lia.
+      + rewrite Nat.ltb_ge in Hlt.
+        apply Forall_cons;
+          rewrite app_length in *; cbn [List.length] in *;
+            replace (S (length l + length acc)) with (length l + n)%nat in * by lia.
+        * left; lia.
+        * apply IHl; simpl; try lia.
+          replace (ll mod n)%nat.
+          symmetry; rewrite <- Nat.add_mod_idemp_r at 1 by lia. (* FIXME why does ‘at 2’ not work? *)
+          rewrite Nat.mod_same by lia.
+          reflexivity.
+  Qed.
+
+  Lemma Forall_chunk'_length_pos {A} (l: list A) n:
+    forall acc, Forall (fun c => length c > 0)%nat (chunk' n l acc).
+  Proof.
+    induction l; simpl; intros.
+    - destruct acc; eauto; [].
+      apply Forall_cons; simpl; eauto || lia.
+    - destruct (_ <? _)%nat; eauto; [].
+      apply Forall_cons; rewrite ?app_length; cbn [length];
+        eauto || lia.
+  Qed.
+
+  Lemma Forall_chunk_length_mod {A} (l: list A) n:
+    (0 < n)%nat ->
+    Forall (fun c => length c = n \/ length c = length l mod n)%nat (chunk n l).
+  Proof.
+    intros; apply Forall_chunk'_length_mod; simpl; eauto.
+  Qed.
+
+  Lemma Forall_chunk_length_le {A} (l: list A) n:
+    (0 < n)%nat -> Forall (fun c => 0 < length c <= n)%nat (chunk n l).
+  Proof.
+    intros; eapply Forall_impl; cycle 1.
+    - apply Forall_and;
+        [ apply Forall_chunk_length_mod | apply Forall_chunk'_length_pos ];
+        eauto.
+    - cbv beta.
+      pose proof Nat.mod_upper_bound (length l) n ltac:(lia).
+      intros ? ([-> | ->] & ?); lia.
+  Qed.
+
+  Lemma length_chunk_app {A} (l l' : list A) (n : nat) :
+    (n <> 0)%nat ->
+    (length l mod n)%nat = 0%nat ->
+    length (chunk n (l ++ l')) = length (chunk n l ++ chunk n l').
+  Proof.
+    intros; repeat rewrite ?app_length, ?length_chunk by assumption.
+    rewrite div_up_add_mod by assumption; reflexivity.
+  Qed.
+
+  Open Scope list_scope.
+
+  Lemma chunk_app {A} : forall (l l': list A) n,
+      (n <> 0)%nat ->
+      (length l mod n = 0)%nat ->
+      chunk n (l ++ l') = chunk n l ++ chunk n l'.
+  Proof.
+    intros * Hn Hmod.
+    eapply nth_ext with (d := []) (d' := []); [ | intros idx ].
+    - apply length_chunk_app; assumption.
+    - intros Hidx; eassert (Some _ = Some _) as HS; [ | injection HS; intros Hs; apply Hs ].
+      rewrite <- !nth_error_nth' by assumption.
+      rewrite <- !nth_error_nth' by (rewrite length_chunk_app in Hidx; eassumption).
+      assert (idx < length (chunk n l) \/ length (chunk n l) <= idx)%nat as [Hlt | Hge] by lia;
+        [ rewrite nth_error_app1 | rewrite nth_error_app2 ]; try eassumption.
+      all: rewrite !nth_error_chunk.
+      all: repeat rewrite ?length_chunk, ?app_length, ?div_up_add_mod in Hlt by assumption.
+      all: repeat rewrite ?length_chunk, ?app_length, ?div_up_add_mod in Hidx by assumption.
+      all: repeat rewrite ?length_chunk, ?app_length, ?div_up_add_mod in Hge by assumption.
+      all: rewrite ?length_chunk, ?app_length, ?div_up_add_mod by assumption.
+      all: try lia.
+      all: pose proof Nat.div_up_range (length l) n ltac:(lia).
+      + pose proof div_up_exact_mod (length l) n ltac:(lia) ltac:(lia).
+        rewrite !firstn_skipn_comm, !firstn_app.
+        replace (idx * n + n - length l)%nat with 0%nat by nia.
+        simpl; rewrite app_nil_r; reflexivity.
+      + rewrite Nat.mul_sub_distr_r.
+        erewrite div_up_exact_mod by lia.
+        rewrite skipn_app, skipn_all2; [ reflexivity | nia ].
+  Qed.
+End Chunks.
+
+Require Import coqutil.Word.LittleEndianList.
+Arguments le_combine: simpl nomatch.
+Arguments le_split : simpl nomatch.
+Arguments Z.mul: simpl nomatch.
+
+Section combine_split.
+  Lemma le_combine_app bs1 bs2:
+    le_combine (bs1 ++ bs2) =
+      Z.lor (le_combine bs1) (Z.shiftl (le_combine bs2) (Z.of_nat (List.length bs1) * 8)).
+  Proof.
+    induction bs1; cbn -[Z.shiftl Z.of_nat Z.mul]; intros.
+    - rewrite Z.mul_0_l, Z.shiftl_0_r; reflexivity.
+    - rewrite IHbs1, Z.shiftl_lor, Z.shiftl_shiftl, !Z.lor_assoc by lia.
+      f_equal; f_equal; lia.
+  Qed.
+
+  Lemma le_combine_0 n:
+    le_combine (repeat Byte.x00 n) = 0.
+  Proof. induction n; simpl; intros; rewrite ?IHn; reflexivity. Qed.
+
+  Lemma le_combine_app_0 bs n:
+    le_combine (bs ++ repeat Byte.x00 n) = le_combine bs.
+  Proof.
+    rewrite le_combine_app; simpl; rewrite le_combine_0.
+    rewrite Z.shiftl_0_l, Z.lor_0_r.
+    reflexivity.
+  Qed.
+
+  Lemma le_combine_snoc_0 bs:
+    le_combine (bs ++ [Byte.x00]) = le_combine bs.
+  Proof. apply le_combine_app_0 with (n := 1%nat). Qed.
+
+  Lemma le_split_mod z n:
+    le_split n z = le_split n (z mod 2 ^ (Z.of_nat n * 8)).
+  Proof.
+    apply le_combine_inj.
+    - rewrite !length_le_split; reflexivity.
+    - rewrite !le_combine_split.
+      Z.push_pull_mod; reflexivity.
+  Qed.
+
+  Lemma split_le_combine' bs n:
+    List.length bs = n ->
+    le_split n (le_combine bs) = bs.
+  Proof. intros <-; apply split_le_combine. Qed.
+
+  Lemma Z_land_le_combine bs1 : forall bs2,
+      Z.land (le_combine bs1) (le_combine bs2) =
+        le_combine (List.map (fun '(x, y) => byte_land x y) (combine bs1 bs2)).
+  Proof.
+    induction bs1.
+    - reflexivity.
+    - destruct bs2; [ apply Z.land_0_r | ]; cbn -[Z.shiftl] in *.
+      rewrite <- IHbs1, !byte_unsigned_land, !Z.shiftl_land.
+      bitblast.Z.bitblast.
+      assert (l < 0 \/ 8 <= i) as [Hlt | Hge] by lia.
+      + rewrite !(Z.testbit_neg_r _ l) by assumption.
+        rewrite !Bool.orb_false_r; reflexivity.
+      + rewrite !testbit_byte_unsigned_ge by lia.
+        simpl; reflexivity.
+  Qed.
+
+  Definition in_bounds n x :=
+    0 <= x < 2 ^ n.
+
+  Definition forall_in_bounds l n:
+    0 <= n ->
+    (Forall (in_bounds n) l) <-> (forall i, in_bounds n (nth i l 0)).
+  Proof.
+    intros; pose proof Z.pow_pos_nonneg 2 n.
+    rewrite Forall_nth_default' with (d := 0);
+      unfold in_bounds; reflexivity || lia.
+  Qed.
+
+  Lemma le_combine_in_bounds bs n:
+    (length bs <= n)%nat ->
+    in_bounds (8 * Z.of_nat n) (le_combine bs).
+  Proof.
+    unfold in_bounds; intros.
+    pose proof le_combine_bound bs.
+    pose proof Zpow_facts.Zpower_le_monotone 2 (8 * Z.of_nat (length bs)) (8 * Z.of_nat n)
+         ltac:(lia) ltac:(lia); lia.
+  Qed.
+
+  Lemma Forall_le_combine_in_bounds n zs:
+    (0 < n)%nat ->
+    Forall (in_bounds (8 * Z.of_nat n)) (List.map le_combine (chunk n zs)).
+  Proof.
+    intros; eapply Forall_map, Forall_impl.
+    - intros a; apply le_combine_in_bounds.
+    - eapply Forall_impl; [ | apply Forall_chunk_length_le ];
+        simpl; intros; lia.
+  Qed.
+
+  Lemma le_split_0_l z:
+    le_split 0 z = [].
+  Proof. reflexivity. Qed.
+
+  Lemma le_split_0_r n:
+    le_split n 0 = repeat Byte.x00 n.
+  Proof.
+    induction n.
+    - reflexivity.
+    - unfold le_split; fold le_split.
+      rewrite Z.shiftr_0_l, IHn; reflexivity.
+  Qed.
+
+  Open Scope list_scope.
+
+  Lemma le_split_zeroes : forall m n z,
+      0 <= z < 2 ^ (8 * Z.of_nat n) ->
+      le_split (n + m) z = le_split n z ++ le_split m 0.
+  Proof.
+    induction n; cbn -[Z.pow Z.of_nat Z.shiftr]; intros * (Hle & Hlt).
+    - replace z with 0 by lia; reflexivity.
+    - rewrite IHn, !le_split_0_r; try reflexivity; [].
+      rewrite Z.shiftr_div_pow2 by lia; split.
+      + apply Z.div_pos; lia.
+      + replace (8 * Z.of_nat (S n)) with (8 + 8 * Z.of_nat n)%Z in Hlt by lia.
+        rewrite Z.pow_add_r in Hlt by lia.
+        apply Z.div_lt_upper_bound; lia.
+  Qed.
+
+  Lemma flat_map_le_split_combine_chunk:
+    forall bs n,
+      (0 < n)%nat ->
+      (length bs mod n)%nat = 0%nat ->
+      flat_map (le_split n) (List.map le_combine (chunk n bs)) = bs.
+  Proof.
+    intros; rewrite flat_map_concat_map, map_map, map_ext_id, concat_chunk; [reflexivity|].
+    intros * Hin;
+      pose proof (Forall_In (Forall_chunk_length_mod _ n ltac:(lia)) Hin);
+      pose proof (Forall_In (Forall_chunk_length_le _ n ltac:(lia)) Hin);
+      cbv beta in *.
+    rewrite split_le_combine'; reflexivity || lia.
+  Qed.
+
+  Lemma map_unsigned_of_Z_le_combine_4
+        {word : Word.Interface.word 32} {word_ok : word.ok word} bs :
+    List.map (fun z : Z => word.unsigned (word := word) (word.of_Z z))
+             (List.map le_combine (chunk 4 bs)) =
+    List.map le_combine (chunk 4 bs).
+  Proof.
+    rewrite map_ext_id; [ reflexivity | ].
+    intros * Hin%(Forall_In (Forall_le_combine_in_bounds 4 bs ltac:(lia))).
+    apply word.unsigned_of_Z_nowrap; assumption.
+  Qed.
+End combine_split.
+
 Section Array.
   Context {width : Z} {word : Word.Interface.word width} {word_ok : word.ok word}.
   Context {value} {Mem : map.map word value} {Mem_ok : map.ok Mem}.
@@ -1346,10 +1732,31 @@ Section Array.
     rewrite Z.mod_mod; lia.
   Qed.
 
+  Lemma Nat_mod_eq' a n:
+    n <> 0%nat ->
+    a = (n * (a / n) + (a mod n))%nat.
+  Proof.
+    intros; pose proof Nat.mul_div_le a n.
+    rewrite Nat.mod_eq; lia.
+  Qed.
+
+  Lemma Nat_mod_eq'' a n:
+    n <> 0%nat ->
+    (n * (a / n) = a - (a mod n))%nat.
+  Proof.
+    intros; pose proof Nat.mul_div_le a n.
+    rewrite Nat.mod_eq; lia.
+  Qed.
+
   Lemma Z_mod_eq' a b:
     b <> 0 ->
+    a = b * (a / b) + a mod b.
+  Proof. pose proof Z.mod_eq a b; lia. Qed.
+
+  Lemma Z_mod_eq'' a b:
+    b <> 0 ->
     b * (a / b) = a - a mod b.
-  Proof. intros H; pose proof Z.mod_eq a b H; lia. Qed.
+  Proof. pose proof Z.mod_eq a b; lia. Qed.
 
   Definition no_aliasing {A} (repr: word -> A -> Mem -> Prop) :=
     (forall a b p delta m R,
@@ -1393,7 +1800,7 @@ Section Array.
       subst base max_len_bytes max_len; rewrite Z2Nat.id by ZnWords.
       rewrite word.unsigned_sub, word.unsigned_add, word.unsigned_of_Z.
       unfold word.wrap; Z.push_pull_mod.
-      rewrite Z_mod_eq'.
+      rewrite Z_mod_eq''.
       match goal with
       | [  |- _ <= ?t < _ ] => replace t with (2 ^ width mod word.unsigned size mod 2 ^ width)
       end.
